WIP formulation

ptranalysis/Ptranalysis/Lalloc.lean
@@ -8,28 +8,136 @@ abbrev Addr := Nat
 abbrev Val := Addr
 abbrev AllocSite := Nat
 
-inductive ControlPrim : Type where
-  | skip : ControlPrim
-  | assign (vto : Var) (vfrom : Var) : ControlPrim
-  | alloc (l: AllocSite) (vto : Var) : ControlPrim
-  | seq (fst : ControlPrim) (snd : ControlPrim) : ControlPrim
+inductive PrimControl : Type where
+  | skip : PrimControl
+  | assign (vto : Var) (vfrom : Var) : PrimControl
+  | alloc (l: AllocSite) (vto : Var) : PrimControl
+  | seq (fst : PrimControl) (snd : PrimControl) : PrimControl
 
-def sitesOf : ControlPrim -> Set AllocSite
-  | ControlPrim.skip => ∅
-  | ControlPrim.assign _ _ => ∅
-  | ControlPrim.alloc l _ => {l}
-  | ControlPrim.seq fst snd => sitesOf fst ∪ sitesOf snd
+open PrimControl
 
-inductive WellFormed : ControlPrim -> Prop where
-  | skipWF : WellFormed ControlPrim.skip
-  | assignWF {vto vfrom} : WellFormed (ControlPrim.assign vto vfrom)
-  | allocWF {l vto} : WellFormed (ControlPrim.alloc l vto)
-  | seqWF {fst snd} : WellFormed fst → WellFormed snd → Disjoint (sitesOf fst) (sitesOf snd) → WellFormed (ControlPrim.seq fst snd)
+@[simp]
+def sitesOf : PrimControl → Set AllocSite
+  | skip => ∅
+  | assign _ _ => ∅
+  | alloc l _ => {l}
+  | seq fst snd => sitesOf fst ∪ sitesOf snd
+
+inductive WellFormed : PrimControl → Prop where
+  | skipWF : WellFormed skip
+  | assignWF {vto vfrom} : WellFormed (assign vto vfrom)
+  | allocWF {l vto} : WellFormed (alloc l vto)
+  | seqWF {fst snd} :
+      WellFormed fst →
+      WellFormed snd →
+      Disjoint (sitesOf fst) (sitesOf snd) →
+      WellFormed (seq fst snd)
+
+open WellFormed
 
 structure WFControl : Type where
-  prim : ControlPrim
+  prim : PrimControl
   wf : WellFormed prim
 
-abbrev Heap := Addr → Option (Val × AllocSite)
-abbrev Stack := (Var → Val)
-abbrev State := (Heap × Stack)
+structure HeapObj : Type where
+  val : Option Val
+  id : AllocSite
+
+abbrev Heap := Addr → Option HeapObj
+abbrev Stack := Var → Option Val
+
+structure State : Type where
+  H : Heap
+  σ : Stack
+
+abbrev StepState := WFControl × State
+
+@[simp]
+def emptyState : State := ⟨fun _ => none, fun _ => none⟩
+
+@[simp]
+def writeMap {β} (map : Var → β) (k : Var) (v : β) : Var → β :=
+  fun k' => if k = k' then v else map k'
+
+@[simp]
+def unallocated (h : Heap) (addr : Addr) : Prop := h addr = none
+
+-- lemma stepPreservesWF : ∀ {c1 c2 c1' s s'},
+--   WellFormed c1 → Step (c1, s) (c1', s') → WellFormed c1'
+
+-- All leaves are automatically well-formed
+@[simp]
+def skipWFControl : WFControl := ⟨skip, skipWF⟩
+@[simp]
+def assignWFControl (vto : Var) (vfrom : Var) : WFControl := ⟨assign vto vfrom, assignWF⟩
+@[simp]
+def allocWFControl (l : AllocSite) (vto : Var) : WFControl := ⟨alloc l vto, allocWF⟩
+
+-- To construct a well-formed sequence, we need to supply a proof that the sites of the two sub-commands are disjoint
+@[simp]
+def wfToControl {c} (wf : WellFormed c) : WFControl := ⟨c, wf⟩
+
+lemma skipLSeqWF {c} (wf : WellFormed c) : WellFormed (seq skip c) := by
+  apply seqWF
+  . exact skipWF
+  . exact wf
+  . simp
+
+-- Small-step semantics of Lalloc
+inductive Step : StepState → StepState → Prop where
+  | seqL : ∀ {c1 c2 c1' : WFControl} {s s' : State},
+      (wf_c1c2 : WellFormed (seq c1.prim c2.prim)) →
+      (wf_c1'c2 : WellFormed (seq c1'.prim c2.prim)) →
+      Step (c1, s) (c1', s') →
+      Step (wfToControl wf_c1c2, s) (wfToControl wf_c1'c2, s')
+  | seqR : ∀ {c : WFControl} {s : State},
+      Step (wfToControl (skipLSeqWF c.wf), s) (c, s)
+  | assign : ∀ {vto vfrom : Var} {h : Heap} {σ σ' : Stack},
+      σ' = writeMap σ vto (σ vfrom) →
+      Step (assignWFControl vto vfrom, ⟨h, σ⟩) (skipWFControl, ⟨h, σ'⟩)
+  | alloc : ∀ {l : AllocSite} {addr : Addr} {vto : Var} {h h' : Heap} {σ σ' : Stack},
+      unallocated h addr →
+      h' = writeMap h addr (some ⟨none, l⟩) →
+      σ' = writeMap σ vto addr →
+      Step (allocWFControl l vto, ⟨h, σ⟩) (skipWFControl, ⟨h', σ'⟩)
+
+inductive StepClosure : StepState → StepState → Prop where
+  | refl : ∀ {st}, StepClosure st st
+  | step : ∀ {st st' st''}, Step st st' → StepClosure st' st'' → StepClosure st st''
+
+-- # Concrete pointer analysis
+
+@[simp]
+def reachable (program : WFControl) (state : State) : Prop :=
+  ∃ program', StepClosure (program, emptyState) (program', state)
+
+@[simp]
+def concretePointsTo (program : WFControl) (v : Var) (site : AllocSite) : Prop :=
+  ∃ (S : State) (p : AllocSite),
+    reachable program S →
+    S.σ v = p ->
+    match (S.H p) with
+      | none => false
+      | some hObj => hObj.id = site
+
+-- # Abstract pointer analysis
+
+abbrev PTAnalysis := WFControl → Var → AllocSite → Prop
+
+@[simp]
+def soundApprox (concrete : PTAnalysis) (abstract : PTAnalysis) : Prop :=
+  ∀ {p : WFControl} {v : Var} {site : AllocSite},
+    concrete p v site -> abstract p v site
+
+infix:51 " ≼ " => soundApprox
+
+-- ## Andersen-style points-to analysis
+
+def PTAlloc (p : WFControl) (var : Var) (site : AllocSite) : Prop :=
+  match p.prim with
+  | alloc l vto => vto = var ∧ l = site
+  | seq fst snd => PTAlloc (wfToControl fst.wf) var site ∨ PTAlloc (wfToControl snd.wf) var site
+  | _ => false
+
+inductive AndersenPointsTo : PTAnalysis where
+  | alloc : ∀ {var : Var} {site : AllocSite}
